some cleanup

src/core/DY.Core.Trace.Experiments.fst
@@ -8,94 +8,8 @@ module B = DY.Core.Bytes
 open DY.Core.Label.Type
 open DY.Core.Trace.Type
 
-#set-options "--fuel 1 --ifuel 1"
+#set-options "--fuel 2 --ifuel 1"
 
-val init_is_prefix:
-  tr:trace{Snoc? tr} ->
-  Lemma 
-  (let Snoc init _ = tr in
-    init <$ tr
-  )
-let init_is_prefix tr =
-    reveal_opaque (`%grows) (grows);
-    norm_spec [zeta; delta_only [`%prefix]] (prefix)
-    
-let rec trace_concat tr1 tr2 =
-  match tr2 with
-  | Nil -> tr1
-  | Snoc init2 ev2 ->
-      Snoc (trace_concat tr1 init2) ev2
-      
-
-val trace_concat_grows:
-  tr1:trace -> tr2:trace ->
-  Lemma (tr1 <$ trace_concat tr1 tr2)
-//  [SMTPat (trace_concat tr1 tr2)]
-let rec trace_concat_grows tr1 tr2 =
-    reveal_opaque (`%grows) (grows);
-    norm_spec [zeta; delta_only [`%prefix]] (prefix);
-    match tr2 with
-    | Nil -> ()
-    | Snoc init ev -> 
-           trace_concat_grows tr1 init
-
-#push-options "--fuel 2"
-val no_set_state_entry_for_concat:
-  p:principal -> sid:state_id ->
-  tr1: trace -> tr2:trace ->
-  Lemma
-    (requires 
-        no_set_state_entry_for p sid tr1
-      /\ no_set_state_entry_for p sid tr2
-    )
-    (ensures
-      no_set_state_entry_for p sid (tr1 `trace_concat` tr2)
-    )
-    // [SMTPat (no_set_state_entry_for p sid tr1)
-    // ; SMTPat (no_set_state_entry_for p sid tr2)]
-let rec no_set_state_entry_for_concat p sid tr1 tr2 =
-  match tr2 with
-  | Nil -> ()
-  | Snoc init2 ev2 -> 
-    init_is_prefix tr2;
-    assert(event_exists tr2 ev2);
-    no_set_state_entry_for_prefix p sid init2 tr2;
-    no_set_state_entry_for_concat p sid tr1 init2
-#pop-options
-
-#push-options "--fuel 2"
-val suffix_after_concat:
-  tr1:trace -> tr2:trace {tr1 <$ tr2} -> tr3:trace{tr2 <$ tr3} ->
-  Lemma
-  ( tr3 `suffix_after` tr1 == (tr2 `suffix_after` tr1) `trace_concat` (tr3 `suffix_after` tr2)
-  )
-let rec suffix_after_concat tr1 tr2 tr3 =     
-  reveal_opaque (`%grows) (grows);
-  norm_spec [zeta; delta_only [`%prefix]] (prefix);
-  match tr3 with
-  | Nil -> ()
-  | Snoc init ev -> 
-      if length tr2 = length tr3
-        then ()
-        else suffix_after_concat tr1 tr2 init
-#pop-options
-
-val no_set_state_entry_for_suffixes_transitive:
-  p:principal -> sid:state_id ->
-  tr1:trace -> tr2:trace{tr1 <$ tr2} -> tr3:trace{tr2 <$ tr3} ->
-  Lemma
-  (requires
-      no_set_state_entry_for p sid (tr2 `suffix_after` tr1)
-    /\ no_set_state_entry_for p sid (tr3 `suffix_after` tr2)
-  )
-  (ensures
-    no_set_state_entry_for p sid (tr3 `suffix_after` tr1)
-  )
-let no_set_state_entry_for_suffixes_transitive p sid tr1 tr2 tr3 =
-  suffix_after_concat tr1 tr2 tr3;
-  no_set_state_entry_for_concat p sid (tr2 `suffix_after` tr1) (tr3 `suffix_after` tr2)
-
-#push-options "--fuel 2"
 let _ = 
   let p = "p" in
   let sid = {the_id = 1} in
@@ -106,7 +20,6 @@ let _ =
   assert(get_event_at tr' 0 = SetState p sid b);
   assert(~(no_set_state_entry_for p sid tr'));
   assert(no_set_state_entry_for "b" sid tr')
-#pop-options
 
 val suffix_after_event:
   ev:trace_event -> tr:trace{event_exists tr ev} -> trace
@@ -117,7 +30,6 @@ let rec suffix_after_event the_ev tr =
         then Snoc (suffix_after_event the_ev init) ev
         else Nil
 
-#push-options "--fuel 2"
 let _ =
   let ev1 = MsgSent (BT.Literal FStar.Seq.Base.empty) in
   let ev2 = Corrupt "p" {the_id = 1} in
@@ -126,10 +38,8 @@ let _ =
   assert(suffix_after_event ev1 tr = Snoc Nil ev2);
   let tr' = Snoc (Snoc (Snoc Nil ev1) ev1) ev2 in  
   assert(suffix_after_event ev1 tr' = Snoc Nil ev2)
-#pop-options
 
 
-#push-options "--fuel 2"
 val get_state_aux_returns_last_set_state : 
   p:principal -> sid:state_id -> tr:trace ->
   Lemma
@@ -154,7 +64,6 @@ let rec get_state_aux_returns_last_set_state p sid tr =
              assert(event_exists init (SetState p sid v));
              get_state_aux_returns_last_set_state p sid init
     end
-#pop-options
 
 val get_state_returns_last_set_state : 
   p:principal -> sid:state_id -> tr:trace ->
