src/core/DY.Core.fst
@@ -108,6 +108,7 @@ include DY.Core.Attacker.Knowledge
 include DY.Core.Label
 include DY.Core.Label.Type
 include DY.Core.Label.Derived
+include DY.Core.Trace.State.Aux
 include DY.Core.Trace.Invariant
 include DY.Core.Trace.Manipulation
 include DY.Core.Trace.Type
@@ -115,5 +116,3 @@ include DY.Core.Trace.Type
 include DY.Core.Bytes
 include DY.Core.Bytes.Type
 
-//include DY.Core.Trace.Experiments
-include DY.Core.Trace.State.Aux
